soundness failed attempt

src/nextgen_soundness.v
@@ -126,374 +126,165 @@ Proof.
   intros m P1 P2 Hm. apply fupd_ne, later_ne, fupd_ne, IHn =>//.
 Qed.
 
-(* Section bnextgen_pred_imod. *)
-(*   Context {M : ucmra} {A : Type} (f : A -> M → M) `{!forall a, CmraMorphism (f a)} {num_laters_per_step : nat -> nat} *)
-(*     `{BiFUpd (uPredI M)}. *)
+Section bnextgen_pred_imod.
+  Context {M : ucmra} {A : Type} (f : A -> M → M) `{!forall a, CmraMorphism (f a)} {num_laters_per_step : nat -> nat}
+    `{BiFUpd (uPredI M)}.
+
+  Fixpoint bnextgen_n
+    (l : list A) (start : nat) (P : uPredI M) : uPredI M :=
+    match l with
+    | [] => P
+    | a :: l' => |={⊤,∅}=> |={∅}▷=>^(S $ num_laters_per_step start) |={∅,⊤}=>
+        ⚡={f a}=> (bnextgen_n l' (S start) P)
+    end.
   
-(*   Notation "P ⊢ Q" := (@uPred_entails M P%I Q%I) : stdpp_scope. *)
-(*   Notation "⊢ Q" := (bi_entails (PROP:=uPredI M) True Q). *)
-(*   Notation "(⊢)" := (@uPred_entails M) (only parsing) : stdpp_scope. *)
-  
-(*   Local Arguments uPred_holds {_} !_ _ _ /. *)
+  Fixpoint bnextgen_n_open
+    (l : list A) (start : nat) (P : uPredI M) : uPredI M :=
+    match l with
+    | [] =>  P
+    | a :: l' => |={⊤,∅}=> |={∅}▷=>^(S $ num_laters_per_step start)
+                          ⚡={f a}=> (bnextgen_n_open l' (S start) P)
+    end.
 
-(*   Ltac unseal := try uPred.unseal; rewrite !uPred_bnextgen_unseal !/uPred_holds /=. *)
+  Notation "⚡={[ l ]}▷=>^ ( n ) P" := (bnextgen_n l n P)
+         (at level 99, l at level 50, n at level 50, P at level 200, format "⚡={[ l ]}▷=>^ ( n )  P") : bi_scope.
 
-(*   Fixpoint bnextgen_n *)
-(*     (l : list A) (start : nat) (P : uPredI M) : uPredI M := *)
-(*     match l with *)
-(*     | [] => P *)
-(*     | a :: l' => |={⊤,∅}=> |={∅}▷=>^(S $ num_laters_per_step start) |={∅,⊤}=> *)
-(*         ⚡={f a}=> (bnextgen_n l' (S start) P) *)
-(*     end. *)
-  
-(*   Fixpoint bnextgen_n_open *)
-(*     (l : list A) (start : nat) (P : uPredI M) : uPredI M := *)
-(*     match l with *)
-(*     | [] =>  |={⊤,∅}=> P *)
-(*     | a :: l' => |={⊤,∅}=> |={∅}▷=>^(S $ num_laters_per_step start) *)
-(*                           ⚡={f a}=> (bnextgen_n_open l' (S start) P) *)
-(*     end. *)
-
-(*   Notation "⚡={[ l ]}▷=>^ ( n ) P" := (bnextgen_n l n P) *)
-(*          (at level 99, l at level 50, n at level 50, P at level 200, format "⚡={[ l ]}▷=>^ ( n )  P") : bi_scope. *)
-
-(*   Notation "⚡={[ l ]}▷=>>^ ( n ) P" := (bnextgen_n_open l n P) *)
-(*          (at level 99, l at level 50, n at level 50, P at level 200, format "⚡={[ l ]}▷=>>^ ( n )  P") : bi_scope. *)
+  Notation "⚡={[ l ]}▷=>>^ ( n ) P" := (bnextgen_n_open l n P)
+         (at level 99, l at level 50, n at level 50, P at level 200, format "⚡={[ l ]}▷=>>^ ( n )  P") : bi_scope.
 
  
-(*   Lemma bnextgen_n_mono P Q l n : *)
-(*     (P ⊢ Q) → (⚡={[ l ]}▷=>^(n) P) ⊢ (⚡={[ l ]}▷=>^(n) Q). *)
-(*   Proof. *)
-(*     intros Hi. revert n; induction l =>n;auto. *)
-(*     iIntros "H". simpl. *)
-(*     iMod "H". iModIntro. *)
-(*     iApply (step_fupdN_mono with "H"). iIntros "H". *)
-(*     iMod "H". iModIntro. iApply (bnextgen_mono with "H"). iApply IHl. *)
-(*   Qed. *)
+  Lemma bnextgen_n_mono P Q l n :
+    (P ⊢ Q) → (⚡={[ l ]}▷=>^(n) P) ⊢ (⚡={[ l ]}▷=>^(n) Q).
+  Proof.
+    intros Hi. revert n; induction l =>n;auto.
+    iIntros "H". simpl.
+    iMod "H". iModIntro.
+    iApply (step_fupdN_mono with "H"). iIntros "H".
+    iMod "H". iModIntro. iApply (bnextgen_mono with "H"). iApply IHl.
+  Qed.
 
-(*   (* Lemma bnextgen_n_mono_keep P Q l n : *) *)
-(*   (*   ((|={⊤}=> P) ⊢ |={⊤}=> Q) → (⚡={[ l ]}▷=>^(n) P) ⊢ (⚡={[ l ]}▷=>^(n) Q). *) *)
-(*   (* Proof. *) *)
-(*   (*   intros Hi. revert n; induction l =>n;auto. *) *)
-(*   (*   { simpl. } *) *)
-(*   (*   iIntros "H". simpl. *) *)
-(*   (*   iMod "H". iModIntro. *) *)
-(*   (*   iApply (step_fupdN_mono with "H"). iIntros "H". *) *)
-(*   (*   iMod "H". iModIntro. iApply (bnextgen_mono with "H"). iApply IHl. *) *)
-(*   (* Qed. *) *)
+  Lemma bnextgen_n_open_mono P Q l n :
+    (P ⊢ Q) → (⚡={[ l ]}▷=>>^(n) P) ⊢ (⚡={[ l ]}▷=>>^(n) Q).
+  Proof.
+    intros Hi. revert n; induction l =>n;auto.
+    iIntros "H". simpl.
+    iMod "H". iModIntro.
+    iApply (step_fupdN_mono with "H"). iIntros "H".
+    iModIntro. iApply IHl. auto.
+  Qed.
 
-(*   Global Instance bnextgen_n_mono' l n : *)
-(*     Proper ((⊢) ==> (⊢)) (bnextgen_n l n). *)
-(*   Proof. intros P Q. apply bnextgen_n_mono. Qed. *)
+  Global Instance bnextgen_n_mono' l n :
+    Proper ((⊢) ==> (⊢)) (bnextgen_n l n).
+  Proof. intros P Q. apply bnextgen_n_mono. Qed.
 
-(*   Global Instance nextgen_n_ne l n : NonExpansive (bnextgen_n l n). *)
-(*   Proof. *)
-(*     revert n; induction l =>n;simpl;auto;try apply _. *)
-(*     (* { apply fupd_ne. } *) *)
-(*     intros x P Q Hne. *)
-(*     destruct H with a. simpl in *. *)
-(*     apply fupd_ne. *)
-(*     apply fupd_ne,later_ne, fupd_ne. *)
-(*     apply step_fupdN_ne. apply fupd_ne. *)
-(*     apply bnextgen_ne.  apply IHl. auto. *)
-(*   Qed. *)
+  Global Instance bnextgen_n_open_mono' l n :
+    Proper ((⊢) ==> (⊢)) (bnextgen_n_open l n).
+  Proof. intros P Q. apply bnextgen_n_open_mono. Qed.
 
-(*   Global Instance bnextgen_n_proper l n : *)
-(*     Proper ((≡) ==> (≡)) (bnextgen_n l n) := ne_proper _. *)
+  Global Instance nextgen_n_ne l n : NonExpansive (bnextgen_n l n).
+  Proof.
+    revert n; induction l =>n;simpl;auto;try apply _.
+    (* { apply fupd_ne. } *)
+    intros x P Q Hne.
+    destruct H with a. simpl in *.
+    apply fupd_ne.
+    apply fupd_ne,later_ne, fupd_ne.
+    apply step_fupdN_ne. apply fupd_ne.
+    apply bnextgen_ne.  apply IHl. auto.
+  Qed.
 
-(*   Lemma bnextgen_n_open_snoc l x n P : *)
-(*     (⚡={[(l ++ [x])]}▷=>>^(n) P) ⊣⊢ ⚡={[l]}▷=>>^(n) (|={∅}▷=> |={∅}▷=>^(num_laters_per_step (n + length l)) ⚡={f x}=> |={⊤,∅}=> P). *)
-(*   Proof. *)
-(*     revert n; induction l => n. *)
-(*     - simpl. iSplit; iIntros "H"; rewrite Nat.add_0_r; auto. *)
-(*     - simpl. iSplit;iIntros ">H". *)
-(*       all: iModIntro. *)
-(*       all: iApply (step_fupdN_mono with "H"); iIntros "H". *)
-(*       all: iApply (bnextgen_mono with "H"); iIntros "H". *)
-(*       + iDestruct (IHl with "H") as "H". *)
-(*         rewrite Nat.add_succ_r. iFrame. *)
-(*       + iApply IHl. rewrite Nat.add_succ_r. iFrame. *)
-(*   Qed. *)
+  Global Instance bnextgen_n_proper l n :
+    Proper ((≡) ==> (≡)) (bnextgen_n l n) := ne_proper _.
 
-(*   Lemma bnextgen_n_snoc l x n P : *)
-(*     (⚡={[(l ++ [x])]}▷=>^(n) P) ⊣⊢ ⚡={[l]}▷=>^(n) (|={⊤,∅}=> |={∅}▷=> |={∅}▷=>^(num_laters_per_step (n + length l)) |={∅,⊤}=> ⚡={f x}=> P). *)
-(*   Proof. *)
-(*     revert n; induction l => n. *)
-(*     - simpl. iSplit; iIntros "H"; rewrite Nat.add_0_r; auto. (* rewrite fupd_trans. auto. *) *)
-(*     - simpl. iSplit;iIntros ">H". *)
-(*       all: iModIntro. *)
-(*       all: iApply (step_fupdN_mono with "H"); iIntros "H". *)
-(*       all: iApply (bnextgen_mono with "H"); iIntros "H". *)
-(*       + iDestruct (IHl with "H") as "H". *)
-(*         rewrite Nat.add_succ_r. iFrame. *)
-(*       + iApply IHl. rewrite Nat.add_succ_r. iFrame. *)
-(*   Qed. *)
+  Lemma bnextgen_n_open_snoc l x n P :
+    (⚡={[(l ++ [x])]}▷=>>^(n) P) ⊣⊢ ⚡={[l]}▷=>>^(n) (|={⊤,∅}=> |={∅}▷=> |={∅}▷=>^(num_laters_per_step (n + length l)) ⚡={f x}=> P).
+  Proof.
+    revert n; induction l => n.
+    - simpl. iSplit; iIntros "H"; rewrite Nat.add_0_r; auto.
+    - simpl. iSplit;iIntros ">H".
+      all: iModIntro.
+      all: iApply (step_fupdN_mono with "H"); iIntros "H".
+      all: iApply (bnextgen_mono with "H"); iIntros "H".
+      + iDestruct (IHl with "H") as "H".
+        rewrite Nat.add_succ_r. iFrame.
+      + iApply IHl. rewrite Nat.add_succ_r. iFrame.
+  Qed.
 
-(*   Lemma bnextgen_n_mono_open_keep  P Q l n : *)
-(*     ((|={⊤,∅}=> P) ⊢ |={⊤,∅}=> Q) → (⚡={[ l ]}▷=>>^(n) P) ⊢ (⚡={[ l ]}▷=>>^(n) Q). *)
-(*   Proof. *)
-(*     intros Hi. revert n; induction l =>n;auto. *)
-(*     iIntros "H". simpl. *)
-(*     iMod "H". iModIntro. *)
-(*     iApply (step_fupdN_mono with "H"). iIntros "H". *)
-(*     iApply (bnextgen_mono with "H"). iApply IHl. *)
-(*   Qed. *)
+  Lemma bnextgen_n_snoc l x n P :
+    (⚡={[(l ++ [x])]}▷=>^(n) P) ⊣⊢ ⚡={[l]}▷=>^(n) (|={⊤,∅}=> |={∅}▷=> |={∅}▷=>^(num_laters_per_step (n + length l)) |={∅,⊤}=> ⚡={f x}=> P).
+  Proof.
+    revert n; induction l => n.
+    - simpl. iSplit; iIntros "H"; rewrite Nat.add_0_r; auto. (* rewrite fupd_trans. auto. *)
+    - simpl. iSplit;iIntros ">H".
+      all: iModIntro.
+      all: iApply (step_fupdN_mono with "H"); iIntros "H".
+      all: iApply (bnextgen_mono with "H"); iIntros "H".
+      + iDestruct (IHl with "H") as "H".
+        rewrite Nat.add_succ_r. iFrame.
+      + iApply IHl. rewrite Nat.add_succ_r. iFrame.
+  Qed.
 
-(*   Local Fixpoint steps_sum (num_laters_per_step : nat → nat) (start ns : nat) : nat := *)
-(*   match ns with *)
-(*   | O => 0 *)
-(*   | S ns => *)
-(*       S $ num_laters_per_step start + steps_sum num_laters_per_step (S start) ns *)
-(*   end. *)
+  (* Lemma bnextgen_n_mono_open_keep  P Q l n : *)
+  (*   ((|={⊤,∅}=> P) ⊢ |={⊤,∅}=> Q) → (⚡={[ l ]}▷=>>^(n) P) ⊢ (⚡={[ l ]}▷=>>^(n) Q). *)
+  (* Proof. *)
+  (*   intros Hi. revert n; induction l =>n;auto. *)
+  (*   iIntros "H". simpl. *)
+  (*   iMod "H". iModIntro. *)
+  (*   iApply (step_fupdN_mono with "H"). iIntros "H". *)
+  (*   iApply (bnextgen_mono with "H"). iApply IHl. *)
+  (* Qed. *)
 
+End bnextgen_pred_imod.
 
-(*   Fixpoint foo *)
-(*     (l : list A) (start : nat) (P : uPredI M) : uPredI M := *)
-(*     match l with *)
-(*     | [] => P *)
-(*     | a :: l' => |={⊤,∅}=> |={∅}▷=>^(S $ num_laters_per_step start) *)
-(*                           (foo l' (S start) P) *)
-(*     end. *)
+Lemma bnextgen_fupd_elim_no_lc `{!invGpreS Σ} `{Hinv: !invGS_gen HasNoLc Σ} E1 E2 (P : iProp Σ) `{!Plain P} (f : iResUR Σ -> iResUR Σ) `{GenTrans (iResUR Σ) f} :
+  (|={E1,E2}=> ⚡={f}=> P) ⊢ |={E1,E2}=> P.
+Proof.
+  iIntros "Hm".
+  iMod "Hm". iModIntro.
+  iApply bnextgen_plain. eauto.
+Qed.
 
-(*   Lemma foo_snoc l x n P : *)
-(*     foo (l ++ [x]) n P -∗ foo (l) n (|={⊤,∅}=> |={∅}▷=> |={∅}▷=>^(num_laters_per_step (n + length l)) P). *)
-(*   Proof. *)
-(*     revert n; induction l => n. *)
-(*     - simpl. iIntros "H". rewrite Nat.add_0_r. auto. *)
-(*     - simpl. iIntros ">H". *)
-(*       iModIntro. *)
-(*       iApply (step_fupdN_mono with "H"). iIntros "H". *)
-(*       rewrite -PeanoNat.Nat.add_succ_comm. iApply IHl. auto. *)
-(*   Qed. *)
+Section test.
+  Context {A : Type} {Σ : gFunctors} (f : A -> iResUR Σ → iResUR Σ) `{!forall a, CmraMorphism (f a)}
+    {num_laters_per_step : nat -> nat}.
 
-(*   Lemma foo_snoc_inv l x n P : *)
-(*     foo (l) n (|={⊤,∅}=> |={∅}▷=> |={∅}▷=>^(num_laters_per_step (n + length l)) P) ⊣⊢ foo (l ++ [x]) n P. *)
-(*   Proof. *)
-(*     revert n; induction l => n. *)
-(*     - simpl. iSplit; iIntros "H"; rewrite Nat.add_0_r; auto. *)
-(*     - simpl. iSplit; iIntros ">H". *)
-(*       all: iModIntro. *)
-(*       all: iApply (step_fupdN_mono with "H"); iIntros "H". *)
-(*       all: rewrite -PeanoNat.Nat.add_succ_comm; iApply IHl; auto. *)
-(*   Qed. *)
+  Notation "⚡={[ l ]}▷=>^ ( n ) P" := (@bnextgen_n _ _ f _ num_laters_per_step _ l n P)
+         (at level 99, l at level 50, n at level 50, P at level 200, format "⚡={[ l ]}▷=>^ ( n )  P") : bi_scope.
 
-(*   (* Lemma  *) *)
+  Notation "⚡={[ l ]}▷=>>^ ( n ) P" := (@bnextgen_n_open _ _ f _ num_laters_per_step _ l n P)
+         (at level 99, l at level 50, n at level 50, P at level 200, format "⚡={[ l ]}▷=>>^ ( n )  P") : bi_scope.
 
-(*   (* Lemma test P `{!Plain P} (* `{!Absorbing P} *) (* `{BiPlainly (uPredI M)} *) l ns : *) *)
-(*   (*   foo l ns P -∗ (⚡={[l]}▷=>>^(ns) P). *) *)
-(*   (* Proof. *) *)
-(*   (*   revert ns; induction l using rev_ind; intros ns. *) *)
-(*   (*   - simpl. auto. *) *)
-(*   (*   - iIntros "H". rewrite -foo_snoc_inv. *) *)
-(*   (*     rewrite bnextgen_n_snoc. *) *)
-(*   (*     iDestruct (bnextgen_n_snoc with "H") as "H". iIntros "H". *) *)
-      
-(*   (*     iApply IHl. *) *)
-      
-      
-    
-
-(* End bnextgen_pred_imod. *)
-
-(* Section test. *)
-(*   Context {A : Type} {Σ : gFunctors} (f : A -> iResUR Σ → iResUR Σ) `{!forall a, CmraMorphism (f a)} *)
-(*     {num_laters_per_step : nat -> nat}. *)
-
-(*   Notation "⚡={[ l ]}▷=>^ ( n ) P" := (@bnextgen_n _ _ f _ num_laters_per_step _ l n P) *)
-(*          (at level 99, l at level 50, n at level 50, P at level 200, format "⚡={[ l ]}▷=>^ ( n )  P") : bi_scope. *)
-
-(*   Notation "⚡={[ l ]}▷=>>^ ( n ) P" := (@bnextgen_n_open _ _ f _ num_laters_per_step _ l n P) *)
-(*          (at level 99, l at level 50, n at level 50, P at level 200, format "⚡={[ l ]}▷=>>^ ( n )  P") : bi_scope. *)
-
-(*   Lemma step_fupdN_soundness_no_lc `{!invGpreS Σ} (P : iProp Σ) `{!Plain P} n m : *)
-(*     (∀ `{Hinv: !invGS_gen HasNoLc Σ}, £ m ={⊤,∅}=∗ |={∅}▷=>^n P) → *)
-(*     ⊢ P. *)
-(*   Proof. *)
-(*     intros Hiter. *)
-(*     apply (laterN_soundness _  (S n)); simpl. *)
-(*     apply (fupd_soundness_no_lc ⊤ ⊤ _ m)=> Hinv. iIntros "Hc". *)
-(*     iPoseProof (Hiter Hinv) as "H". clear Hiter. *)
-(*     iApply fupd_plainly_mask_empty. iSpecialize ("H" with "Hc"). *)
-(*     iMod (step_fupdN_plain with "H") as "H". iMod "H". iModIntro. *)
-(*     rewrite -later_plainly -laterN_plainly -later_laterN laterN_later. *)
-(*     iNext. iMod "H" as "#H". auto. *)
-(*   Qed. *)
-
-(*   (* Lemma step_fupdN_nextgen_soundness_gen : *) *)
-(*   (*   invGpreS Σ → ∀ P : iProp Σ, *) *)
-(*   (*       Plain P → ∀ (hlc : has_lc) (n m : nat), (∀ (Hinv : invGS_gen hlc Σ) l, £ m ={⊤}=∗ ⚡={[l]}▷=>>^(n) P) → (⊢ P)%stdpp. *) *)
-(*   (* Proof. *) *)
-(*   (*   intros. *) *)
-(*   (*   eapply (fupd_soundness_gen _ hlc m ⊤ ⊤);eauto. *) *)
-(*   (*   intros. specialize H2 with Hinv []. simpl in *. auto. *) *)
-(*   (* Qed. *) *)
-
-
-(*   Lemma test : *)
-(*     invGpreS Σ *)
-(*     → ∀ P : iProp Σ, Plain P → ∀ (n m : nat) l, (∀ Hinv : invGS_gen HasNoLc Σ, *)
-(*                                                   £ m ={⊤}=∗ ⚡={[ l ]}▷=>^(n) P) → (⊢ P)%stdpp. *)
-(*   Proof. *)
-(*     intros. (* apply bupd_soundness;auto. *) *)
-(*     pose proof (step_fupdN_soundness_no_lc P). *)
-
-    
-(*     eapply (step_fupdN_soundness_gen _ HasNoLc ((length l)) m);eauto. *)
-(*     intros. iIntros "Hm". *)
-(*     iDestruct (H2 with "Hm") as "H". clear H2. *)
-(*     iRevert "H". iApply entails_wand. *)
-(*     revert n. induction l. *)
-(*     - simpl. iIntros (n) "H". iMod "H". *)
-(*       iApply fupd_mask_intro;auto. (* iIntros "Hcls". *) *)
-(*       (* iApply step_fupdN_intro;auto. *) *)
-(*     - simpl. intros. iIntros "H". *)
-      
-      
-
-(*       iAssert (|={⊤}=> |={⊤,∅}=> |={∅}▷=> |={∅}▷=>^(num_laters_per_step n) |={∅,⊤}=> ⚡={f a}=> |={⊤,∅}=> |={∅}▷=>^(length l) P)%I with "[H]" as  "H". *)
-(*       { iMod "H". iModIntro. iMod "H". iModIntro. *)
-(*         iApply (step_fupdN_mono with "H"). *)
-(*         iIntros "H". *)
-(*         iMod "H". iModIntro. iModIntro. *)
-(*         iApply IHl. auto. } *)
-      
-      
-      
-(*       iApply IHl. *)
-
-      
-
-(*       intros. auto. *)
-(*     - simpl. intros. iIntros "H". *)
-(*       iAssert (|={⊤}=> |={⊤,∅}=> |={∅}▷=> |={∅}▷=>^(num_laters_per_step n) P)%I with "[H]" as "H". *)
-(*       { iMod "H". iMod "H". *)
-(*         pose proof fupd_soundness_gen. *)
-
-(*         iModIntro. iApply (step_fupdN_mono with "H"). iIntros "H". *)
-(*         iApply bnextgen_plain. iApply (bnextgen_mono with "H"). *)
-(*         iIntros "H". iApply IHl *)
-        
-(*       }  *)
-      
-(*       iMod "H". iMod "H". *)
-(*       iApply fupd_mask_intro_discard. *)
-
-
-    
-(*     intros. *)
-(*     eapply fancy_updates.step_fupdN_soundness_no_lc with (* (hlc := HasNoLc) *) (m:=m) (n := (length l));eauto. *)
-(*     intros. specialize (H2 Hinv). *)
-(*     iIntros "Hm". iDestruct (H2 with "Hm") as "H". *)
-(*     clear H2. (* rewrite step_fupdN_S_fupd.  *)iRevert "H". iApply entails_wand. *)
-(*     revert n Hinv. induction l using rev_ind =>n Hinv. *)
-(*     - simpl. iIntros "Hp". iMod "Hp". *)
-(*       iApply fupd_mask_intro;auto. *)
-(*       (* iIntros "Hcls". iNext. iMod "Hcls". iModIntro. auto. *) *)
-(*     - iIntros "H". rewrite app_length /=. (* rewrite -Nat.add_succ_l. (* simpl. *) *) *)
-(*       (* rewrite PeanoNat.Nat.add_1_r. rewrite bnextgen_n_snoc. simpl. *) *)
-(*       rewrite step_fupdN_add. rewrite bnextgen_n_snoc. destruct l. *)
-
-(*       iApply step_fupdN_mono. *)
-      
-(*       iApply fupd_mask_intro;auto. iIntros "Hcls". iNext. *)
-
-(*       rewrite PeanoNat.Nat.add_1_r. rewrite bnextgen_n_snoc. *)
-(*       iMod "Hcls". *)
-(*       iModIntro. rewrite PeanoNat.Nat.add_1_r. iApply IHl. *)
-(*       rewrite step_fupdN_add /=. *)
-(*       rewrite bnextgen_n_snoc. *)
-
-(*       iAssert ((|={⊤,∅}=> |={∅}▷=>^(length l) P) -∗ *)
-(*                                                    |={⊤,∅}=> |={∅}▷=>^(length l) |={∅}▷=> P)%I as "tes". *)
-(*       { iIntros "H". iMod "H". iModIntro. iApply (step_fupdN_mono with "H"). iIntros "H". *)
-(*         iModIntro. iNext. iModIntro. auto. } *)
-(*       iApply "tes". *)
-      
-(*       iApply (IHl n). iMod "H". iModIntro. *)
-(*       iApply (bnextgen_n_mono with "H"). iIntros "H". *)
-
-(*       iAssert (|={⊤,∅}=> |={∅}▷=> |={∅}▷=>^(num_laters_per_step (n + length l)) |={∅,⊤}=> P)%I with "[H]" as "H". *)
-(*       { iMod "H". iModIntro. iApply (step_fupdN_mono with "H"). iIntros "H". iMod "H". *)
-(*         iModIntro. iApply (bnextgen_plain). eauto. } *)
-
-(*       unseal. simpl. *)
-      
-(*       simpl in IHl. *)
-(*       iApply IHl. *)
-
-    
-(*     intros. (* apply bupd_soundness;auto. *) *)
-(*     eapply (fupd_soundness_gen _ HasNoLc m ⊤ ⊤);eauto. *)
-(*     intros. iIntros "Hm". *)
-(*     iDestruct (H2 with "Hm") as "H". clear H2. *)
-(*     iRevert "H". iApply entails_wand. *)
-(*     revert n. induction l. *)
-(*     - simpl. intros. auto. *)
-(*     - simpl. intros. iIntros "H". *)
-(*       iAssert (|={⊤}=> |={⊤,∅}=> |={∅}▷=> |={∅}▷=>^(num_laters_per_step n) P)%I with "[H]" as "H". *)
-(*       { iMod "H". iMod "H". *)
-(*         pose proof fupd_soundness_gen. *)
-
-(*         iModIntro. iApply (step_fupdN_mono with "H"). iIntros "H". *)
-(*         iApply bnextgen_plain. iApply (bnextgen_mono with "H"). *)
-(*         iIntros "H". iApply IHl *)
-        
-(*       }  *)
-      
-(*       iMod "H". iMod "H". *)
-(*       iApply fupd_mask_intro_discard. *)
-    
-
-(*   Lemma step_fupdN_nextgen_soundness_gen : *)
-(*     invGpreS Σ → ∀ P : iProp Σ, *)
-(*         Plain P → ∀ (hlc : has_lc) (n m : nat), (∀ (Hinv : invGS_gen hlc Σ) l, £ m -∗ ⚡={[l]}▷=>>^(n) P) → (⊢ P)%stdpp. *)
-(*   Proof. *)
-(*     intros. *)
-(*     eapply (fupd_soundness_gen _ hlc m ⊤ ⊤);eauto. *)
-(*     intros. specialize H2 with Hinv []. simpl in *. auto. *)
-(*   Qed. *)
+  Local Fixpoint steps_sum (num_laters_per_step : nat → nat) (start ns : nat) : nat :=
+  match ns with
+  | O => 0
+  | S ns =>
+      S $ num_laters_per_step start + steps_sum num_laters_per_step (S start) ns
+  end.
 
   
 
-(*   Lemma step_fupdN_nextgen_soundness_gen' : *)
-(*     invGpreS Σ → ∀ P : iProp Σ, *)
-(*         Plain P → ∀ l (hlc : has_lc) (n m : nat), (∀ (Hinv : invGS_gen hlc Σ), £ m -∗ ⚡={[l]}▷=>>^(n) P) → (⊢ P)%stdpp. *)
-(*   Proof. *)
-(*     (* induction l;intros. *) *)
-(*     (* - simpl. eapply (fupd_soundness_gen _ hlc m ⊤ ⊤);eauto. *) *)
-(*     (* - simpl in *. eapply IHl. intros. *) *)
-(*     (*   iIntros "Hm". iDestruct (H2 with "Hm") as "H". *) *)
-(*     (*   apply H2. ;eauto. apply H2. *) *)
+  Lemma step_fupdN_nextgen_soundness_no_lc (l : list A) :
+    invGpreS Σ → ∀ P : iProp Σ,
+        Plain P → ∀ (n m : nat), (∀ (Hinv : invGS_gen HasNoLc Σ), £ m -∗ ⚡={[l]}▷=>>^(n) (* |={⊤,∅}=> *) P) → (⊢ P)%stdpp.
+  Proof.
+    intros until m. intros Hiter.
+    apply bupd_soundness;auto.
+    iMod (fupd_soundness_no_lc_unfold (m + (steps_sum num_laters_per_step (S n) (length l))) ⊤) as (Hws ω) "[Hm [Hω #H]]". specialize (Hiter Hws).
+    rewrite lc_split. iDestruct "Hm" as "[Hm Hn]".
+    iDestruct (Hiter with "Hm") as "HH". clear Hiter.
+    remember ⊤ as E. clear HeqE.
+    iInduction l as [|x l] "IH" using rev_ind forall (n E).
+    - simpl in *. auto. (* eapply fupd_soundness_no_lc;eauto. intros. iIntros "Hm". (* iMod (Hiter with "Hm"). iModIntro. auto. *) iApply Hiter. by iFrame.- *)
+    - rewrite app_length /= PeanoNat.Nat.add_1_r /= -plus_Sn_m.
+      rewrite lc_split lc_succ.
+      iDestruct "Hn" as "[[Hone Hm] Hn]".
+      iApply ("IH" with "Hn Hω"). (* intros. iIntros "Hm". *)
+      (* iDestruct (Hiter with "Hm") as "Hm". *)
+      rewrite bnextgen_n_open_snoc.
 
-(*     intros. *)
-(*     eapply (fupd_soundness_gen _ hlc m ⊤ ⊤);eauto. *)
-(*     intros. specialize H2 with Hinv. *)
-(*     iIntros "Hm". iDestruct (H2 with "Hm") as "H". *)
-(*     iRevert "H". iApply wand_entails. *)
-(*     clear H2. revert n. induction l;intros. *)
-(*     - simpl in *. iIntros ">H". auto. *)
-(*     - simpl. iIntros "H". iApply (IHl (S n)). *)
-
-(*       lc_fupd_elim_later *)
-
-
-    
-(*     revert n. induction l using rev_ind;intros. *)
-(*     - simpl in *. iIntros ">H". auto. (* eapply fupd_soundness_gen;eauto. *) *)
-(*     - apply (laterN_soundness _  (S 0)); simpl. iIntros "H". iDestruct (bnextgen_n_snoc with "H") as "H". *)
-(*       iApply IHl. iApply (bnextgen_n_mono_open_keep with "H"). *)
-(*       iIntros "H". iMod "H". iApply fupd_plainly_mask_empty. *)
-(*       iMod "H". iMod "H". rewrite -later_plainly.  -laterN_plainly -later_laterN laterN_later. *)
-
-(*       iModIntro. iApply fupd_mask_intro. iModIntro. *)
-
-(*       apply IHl. intros. specialize H2 with Hinv. *)
-(*       iIntros "Hm". iDestruct (H2 with "Hm") as "H". *)
-(*       iDestruct (bnextgen_n_snoc with "H") as "H". *)
-(*       iApply (bnextgen_n_mono_open_keep with "H"). *)
-(*       iIntros "H". iMod "H". iModIntro. *)
-      
-      
+      iAssert (⚡={[l]}▷=>>^(n) P)%I with "[HH]" as "test".
+      { iApply (bnextgen_n_open_mono with "HH"). iIntros "H". admit. }
+  Abort. 
     
 
-(* End test. *)
+End test.
